Write first part of read_fill spec
Reorganized function into prepare and then rest, since prepare is the
smallest atomic unit that preserves the invariant.

Writing the spec exposed several bugs throughout specs and protocol.
Getting the proof to a reasonable state added a few theorems and fixed
problems with the automation.

src/ConcurrentCache.v
@@ -50,20 +50,37 @@ Section ConcurrentCache.
       wb_rep (get vDisk0 s) (get vWriteBuffer s) (get vdisk s) /\
       no_wb_reader_conflict (get vCache s) (get vWriteBuffer s).
 
+  (** a locking-like protocol, but true for any provable program
+      due to the program semantics themselves *)
+  Definition readers_locked tid (vd vd': DISK) :=
+      (forall a v tid', vd a = Some (v, Some tid') ->
+                   tid <> tid' ->
+                   vd' a = Some (v, Some tid')).
+
+  Lemma readers_locked_refl : forall tid vd,
+      readers_locked tid vd vd.
+  Proof.
+    unfold readers_locked; eauto.
+  Qed.
+
+  Lemma readers_locked_trans : forall tid vd vd' vd'',
+      readers_locked tid vd vd' ->
+      readers_locked tid vd' vd'' ->
+      readers_locked tid vd vd''.
+  Proof.
+    unfold readers_locked; eauto.
+  Qed.
+
   (* not sure whether to say this about vDisk0, vDisk, or both *)
   Definition cacheR (tid:TID) : Relation Sigma :=
     fun s s' =>
       let vd := get vDisk0 s in
       let vd' := get vDisk0 s' in
       same_domain vd vd' /\
-      (* a locking-like protocol, but true for any provable program
-      due to the program semantics themselves *)
-      (forall a v tid', vd a = Some (v, Some tid') ->
-                   tid <> tid' ->
-                   vd' a = Some (v, Some tid')).
+      readers_locked tid vd vd'.
 
   Hint Resolve same_domain_refl same_domain_trans.
-  Hint Resolve lock_protocol_refl.
+  Hint Resolve readers_locked_refl readers_locked_trans.
 
   Theorem cacheR_trans_closed : forall tid s s',
       star (cacheR tid) s s' ->
@@ -100,25 +117,24 @@ Section ConcurrentCache.
           rx (cache_val c a)
       end.
 
-  Definition AsyncRead a rx : prog Sigma :=
+  (** Prepare to fill address a, locking the address and marking it
+  invalid in the cache to signal the lock to concurrent threads. *)
+  Definition prepare_fill a rx : prog Sigma :=
     tid <- GetTID;
       _ <- StartRead_upd a;
       (* note that no updates to Disk are needed since the readers are
     hidden *)
       _ <- var_update vDisk0
         (fun vd => add_reader vd a tid);
+      _ <- modify_cache (fun c => cache_add c a Invalid);
+      rx tt.
+
+  Definition cache_fill a rx : prog Sigma :=
+    _ <- prepare_fill a;
       _ <- Yield a;
       v <- FinishRead_upd a;
       _ <- var_update vDisk0
         (fun vd => remove_reader vd a);
-      rx v.
-
-  Definition cache_fill a rx : prog Sigma :=
-      (* invalidating + adding a reader makes the address locked,
-      expressed via a reader locking protocol and restrictions on
-      readers in cache_rep *)
-    _ <- modify_cache (fun c => cache_invalidate c a);
-      v <- AsyncRead a;
       _ <- modify_cache (fun c => cache_add c a (Clean v));
       rx v.
 
@@ -173,18 +189,29 @@ Section ConcurrentCache.
     auto.
   Qed.
 
-  Ltac learn_invariant :=
+  Lemma unfold_protocol : forall tid s s',
+      guar delta tid s s' ->
+      ltac:(let t := eval cbn in (guar delta tid s s') in
+                let t := eval unfold cacheR in t in
+                    exact t).
+  Proof.
+    eauto.
+  Qed.
+
+  Ltac learn_protocol :=
     match goal with
     | [ H: invariant delta _ _ _ |- _ ] =>
       learn that (unfold_invariant H)
+    | [ H: guar delta _ _ _ |- _ ] =>
+      learn that (unfold_protocol H)
     end.
 
   Ltac prove_protocol :=
     match goal with
     | [ |- guar delta ?tid _ _ ] =>
-      cbn; unfold cacheR
+      simpl; unfold cacheR
     | [ |- invariant delta _ _ _ ] =>
-      cbn; unfold cacheI
+      simpl; unfold cacheI
     end.
 
   Ltac descend :=
@@ -228,7 +255,7 @@ Section ConcurrentCache.
   Ltac simplify_step :=
     match goal with
     | [ |- forall _, _ ] => intros
-    | _ => learn_invariant
+    | _ => learn_protocol
     | _ => deex
     | _ => progress destruct_ands
     | _ => inv_opt
@@ -252,12 +279,18 @@ Section ConcurrentCache.
   Ltac simplify :=
     repeat (time "simplify_step" simplify_step).
 
+  (* hook up new finish and simplify to existing hoare tactic; this
+    isn't clean, need better extensibility *)
+
+  Ltac step_simplifier ::= simplify.
+  Ltac step_finisher ::= finish.
+
   (* prove hoare specs *)
 
   Theorem modify_cache_ok : forall up,
       SPEC delta, tid |-
               {{ (_:unit),
-               | PRE d m s0 s: invariant delta d m s
+               | PRE d m s0 s: get mCache m = get vCache s
                | POST d' m' s0' s' r:
                    s' = set vCache (up (get vCache s)) s /\
                    m' = set mCache (up (get mCache m)) m /\
@@ -265,7 +298,7 @@ Section ConcurrentCache.
                    s0' = s0
               }} modify_cache up.
   Proof.
-    hoare pre simplify with finish.
+    hoare.
   Qed.
 
   Hint Extern 1 {{ modify_cache _; _ }} => apply modify_cache_ok : prog.
@@ -273,7 +306,7 @@ Section ConcurrentCache.
   Theorem modify_wb_ok : forall up,
       SPEC delta, tid |-
               {{ (_:unit),
-               | PRE d m s0 s: invariant delta d m s
+               | PRE d m s0 s: get mWriteBuffer m = get vWriteBuffer s
                | POST d' m' s0' s' r:
                    s' = set vWriteBuffer (up (get vWriteBuffer s)) s /\
                    m' = set mWriteBuffer (up (get mWriteBuffer m)) m /\
@@ -281,7 +314,7 @@ Section ConcurrentCache.
                    s0' = s0
               }} modify_wb up.
   Proof.
-    hoare pre simplify with finish.
+    hoare.
   Qed.
 
   Hint Extern 1 {{ modify_wb _; _ }} => apply modify_wb_ok : prog.
@@ -296,15 +329,95 @@ Section ConcurrentCache.
                | POST d' m' s0' s' r:
                    invariant delta d m s /\
                    s0' = s0 /\
-                   forall v, r = Some v ->
-                        v = v0
+                   (forall v, r = Some v ->
+                         v = v0) /\
+                   (r = None ->
+                    cache_val (get vCache s') a = None)
               }} cache_maybe_read a.
   Proof.
-    hoare pre simplify with finish.
-
-    (* for some reason, wb_val_none as a Hint doesn't work, but this
-    does *)
+    hoare.
     eauto using wb_val_none.
   Qed.
+
+  Theorem disk_no_reader : forall d c vd0 wb vd a v,
+      cache_get c a = Missing ->
+      cache_rep d c vd0 ->
+      wb_rep vd0 wb vd ->
+      vd a = Some v ->
+      d a = Some (v, None).
+  Proof.
+    unfold const; intros.
+    specialize (H0 a).
+    specialize (H1 a).
+    simpl_match.
+    destruct matches in *;
+      intuition auto;
+      repeat deex;
+      eauto || congruence.
+  Qed.
+
+  Hint Resolve disk_no_reader.
+
+  Lemma no_wb_reader_conflict_stable_invalidate : forall c wb a,
+      no_wb_reader_conflict c wb ->
+      wb_get wb a = WbMissing ->
+      no_wb_reader_conflict (cache_add c a Invalid) wb.
+  Proof.
+    unfold no_wb_reader_conflict; intros.
+    destruct (weq a a0); subst;
+      autorewrite with cache in *;
+      eauto.
+  Qed.
+
+  Hint Resolve no_wb_reader_conflict_stable_invalidate.
+
+  Lemma same_domain_add_reader : forall d a tid,
+      same_domain d (add_reader d a tid).
+  Proof.
+    unfold same_domain, subset, add_reader; split;
+      intros;
+      destruct (weq a a0); subst;
+        destruct matches in *;
+        autorewrite with upd in *;
+        eauto.
+  Qed.
+
+  Hint Resolve same_domain_add_reader.
+
+  Theorem prepare_fill_ok : forall a,
+      SPEC delta, tid |-
+              {{ v0,
+               | PRE d m s0 s:
+                   invariant delta d m s /\
+                   cache_get (get vCache s) a = Missing /\
+                   (* XXX: not sure exactly why this is a requirement,
+                   but it comes from no_wb_reader_conflict *)
+                   wb_get (get vWriteBuffer s) a = WbMissing /\
+                   get vdisk s a = Some v0 /\
+                   guar delta tid s0 s
+               | POST d' m' s0' s' _:
+                   invariant delta d' m' s' /\
+                   get vDisk0 s' a = Some (v0, Some tid) /\
+                   guar delta tid s0' s'
+              }} prepare_fill a.
+  Proof.
+    hoare.
+    eexists; simplify; finish.
+    eauto using disk_no_reader.
+
+    hoare;
+      match goal with
+      (* cache_rep stable when adding reader *)
+      | [ |- cache_rep (upd _ _ _)
+                      (cache_add _ _ _)
+                      (add_reader _ _ _) ] => admit
+      (* wb_rep insensitive to readers *)
+      | [ |- wb_rep (add_reader _ _ _) _ _ ] => admit
+      (* add_reader -> upd *)
+      | [ |- add_reader _ ?a _ ?a = _ ] => admit
+      (* readers only increased *)
+      | [ |- readers_locked _ _ (add_reader _ _ _) ] => admit
+      end.
+  Admitted.
 
 End ConcurrentCache.
